src/HaclExample.fst
@@ -1,15 +1,40 @@
 module HaclExample
 
+open Hacl.Hash.Definitions
+open Spec.Hash.Definitions
+
+open Lib.IntTypes
+
+open FStar.HyperStack
+open FStar.HyperStack.ST
+
+module HI = Lib.IntTypes
+module B = LowStar.Buffer
+module SHD = Spec.Hash.Definitions
+
 let hash_example
-  (hash: FStar.Buffer.buffer FStar.UInt32.t {FStar.Buffer.length hash = 64})
-  (input:FStar.Buffer.buffer FStar.UInt32.t {FStar.Buffer.length input < pow2 125})
-  (len  :FStar.UInt32.t{FStar.UInt32.v len = FStar.Buffer.length input})
-: FStar.HyperStack.ST.St unit
+  (input:B.buffer HI.uint8)
+  (len  :FStar.UInt32.t{FStar.UInt32.v len = LowStar.Buffer.length input})
+  (hash: Hacl.Hash.Definitions.hash_t Spec.Hash.Definitions.SHA2_512)
+: Stack unit
+  (requires (fun h ->
+      B.live h input /\
+      B.live h hash /\
+      B.disjoint input hash /\
+      B.length input <= SHD.max_input_length SHD.SHA2_512))
+  (ensures fun _ _ _ -> True)
 =
-  FStar.HyperStack.ST.push_frame ();
-  Hacl.SHA2_512.hash
-    hash
+  push_frame ();
+
+  let h
+    : hash_t SHD.SHA2_512
+  =
+    B.alloca (u8 0x00) (hash_len SHD.SHA2_512)
+  in
+
+  Hacl.Hash.SHA2.hash_512
     input
-    len;
-  FStar.HyperStack.ST.pop_frame ();
+    len
+    hash;
+  pop_frame ();
   ()
